src/lib/notation.lean
@@ -30,11 +30,11 @@ lemma numeral_one_def  {α : Type*} [has_zero α] [has_succ α] : (1 : α) = Suc
 
 @[notation_class] class has_exists_quantifier (α : Sort*) := (ex : α → α)
 
-@[notation_class] class has_univ_quantifier' (α : Sort*) (β : Sort*):= (univ : α → β)
+@[notation_class] class has_univ_quantifier' (α : ℕ → Sort*) := (univ : Π {n}, α (n + 1) → α n)
 
-@[notation_class] class has_exists_quantifier' (α : Sort*) (β : Sort*) := (ex : α → β)
+@[notation_class] class has_exists_quantifier' (α : ℕ → Sort*) := (ex : Π {n}, α (n + 1) → α n)
 
-localized "infix (name := has_eq.eq) ` ≃ `:50 := has_eq.eq" in logic_symbol
+localized "infix (name := has_eq.eq) ` =' `:50 := has_eq.eq" in logic_symbol
 localized "infix (name := has_prec.prec) ` ≺ `:50 := has_prec.prec" in logic_symbol
 localized "infix (name := has_preceq.preceq) ` ≼ `:50 := has_preceq.preceq" in logic_symbol
 localized "infix (name := has_elem.elem) ` ∊ `:50 := has_elem.elem" in logic_symbol
@@ -42,15 +42,45 @@ localized "prefix (name := has_negation.neg) `∼`:75 := has_negation.neg" in lo
 localized "infixr (name := has_arrow.arrow) ` ⟶ `:60 := has_arrow.arrow" in logic_symbol
 localized "prefix (name := has_univ_quantifier.univ) `∀. `:64 := has_univ_quantifier.univ" in logic_symbol
 localized "prefix (name := has_exists_quantifier.ex) `∃. `:64 := has_exists_quantifier.ex" in logic_symbol
-localized "prefix (name := has_univ_quantifier'.univ) `∀' `:64 := has_univ_quantifier'.univ" in logic_symbol
-localized "prefix (name := has_exists_quantifier'.ex) `∃' `:64 := has_exists_quantifier'.ex" in logic_symbol
+localized "prefix (name := has_univ_quantifier'.univ) `∀'`:64 := has_univ_quantifier'.univ" in logic_symbol
+localized "prefix (name := has_exists_quantifier'.ex) `∃'`:64 := has_exists_quantifier'.ex" in logic_symbol
 
 open_locale logic_symbol
 
-@[reducible] def has_eq.ineq {α : out_param (Sort*)} {β : Sort*}
-  [has_eq α β] [has_negation β] (a b : α) : β := ∼(a ≃ b)
+section has_univ_quantifier'
+variables  {α : ℕ → Sort*} [has_univ_quantifier' α]
 
-localized "infix (name := has_eq.ineq) ` ≄ `:50 := has_eq.ineq" in logic_symbol
+def nforall {n} : Π (k), α (n + k) → α n
+| 0     a := a
+| (k+1) a := nforall _ ∀'a
+
+def universal_closure : Π {n}, α n → α 0
+| 0     a := a
+| (k+1) a := universal_closure ∀'a
+
+localized "notation (name := universal_closure) `∀'*`:64 := universal_closure" in logic_symbol
+
+end has_univ_quantifier'
+
+section has_exists_quantifier'
+variables {α : ℕ → Sort*} [has_exists_quantifier' α]
+
+def nexists {n} : Π (k), α (n + k) → α n
+| 0     a := a
+| (k+1) a := nexists _ ∃'a
+
+def exists_close : Π {n}, α n → α 0
+| 0     a := a
+| (k+1) a := exists_close ∃'a
+
+localized "notation (name := exists_close) `∃'*`:64 := exists_close" in logic_symbol
+
+end has_exists_quantifier'
+
+@[reducible] def has_eq.ineq {α : out_param (Sort*)} {β : Sort*}
+  [has_eq α β] [has_negation β] (a b : α) : β := ∼(a =' b)
+
+localized "infix (name := has_eq.ineq) ` ≠' `:50 := has_eq.ineq" in logic_symbol
 
 @[notation_class] class has_turnstile (α : Sort*) := (turnstile : set α → α → Prop)
 
